language/move-prover/bytecode-to-boogie/test_mvir/verify-stdlib/libra_account.prover.bpl
@@ -1,0 +1,18 @@
+// Native functions and helpers for libra_account
+
+// TODO: fill in implementation
+
+procedure {:inline 1} LibraAccount_save_account (arg0: Value, arg1: Value) returns ();
+  requires ExistsTxnSenderAccount(m, txn);
+  ensures !abort_flag ==> b#Boolean(ExistsResource(m, LibraAccount_T_type_value(), a#Address(arg0)));
+  ensures !abort_flag ==> b#Boolean(Boolean((Dereference(m, GetResourceReference(LibraAccount_T_type_value(), a#Address(arg0)))) == (arg1)));
+  ensures old(!(b#Boolean(ExistsResource(m, LibraAccount_T_type_value(), a#Address(arg0))))) ==> !abort_flag;
+  ensures old(b#Boolean(ExistsResource(m, LibraAccount_T_type_value(), a#Address(arg0)))) ==> abort_flag;
+
+procedure {:inline 1} LibraAccount_write_to_event_store (tv0: TypeValue, arg0: Value, arg1: Value, arg2: Value) returns ();
+  requires ExistsTxnSenderAccount(m, txn);
+  ensures old(b#Boolean(Boolean(true))) ==> !abort_flag;
+
+function {:inline 1} max_balance(): Value {
+  Integer(9223372036854775807)
+}
