language/move-prover/bytecode-to-boogie/test_mvir/test-specs-translate.prover.bpl
@@ -1,0 +1,9 @@
+// Boogie helper functions for test-specs-translate.mvir
+
+function {:inline} number_in_range(x: Value): Value {
+  Boolean(i#Integer(x) >= 0 && i#Integer(x) < 128)
+}
+
+function {:inline} max_u64(): Value {
+  Integer(MAX_U64)
+}
